used option instead of undefined and implement the remaining stores + some clean-up

BoogieLang/Semantics.thy
@@ -9,8 +9,9 @@ subsection \<open>Values, State, Variable Context\<close>
 text \<open>The values (and as a result the semantics) are parametrized by the carrier type 'a for the 
 abstract values (values that have a type constructed via type constructors)\<close>
 datatype ('a, 'k) val_aux = LitV lit | AbsV (the_absv: 'a)
-  | MapV ty ty "('k, ('a, 'k) val_aux) map" 'k
+  | MapV ty ty "('k, ('a, 'k) val_aux) map" "'k option"
 
+(* user needs to instantiate how many nesting levels to support *)
 type_synonym 'a val0 = "('a, unit)  val_aux"
 type_synonym 'a val1 = "('a, 'a val0) val_aux"
 type_synonym 'a val2 = "('a, 'a val1) val_aux"
@@ -21,48 +22,64 @@ abbreviation IntV where "IntV i \<equiv> LitV (LInt i)"
 abbreviation BoolV where "BoolV b \<equiv> LitV (LBool b)"
 abbreviation RealV where "RealV r \<equiv> LitV (LReal r)"
 
-(* examples *)
+(* MapV examples *)
 value "IntV 1 :: unit val3"
 value "IntV 2 :: unit val4"
-fun m34 :: "unit \<Rightarrow> (unit val3, unit val4) map" where "m34 () = [IntV 1 \<mapsto> IntV 2]"
+definition simple_map_example :: "(unit val3, unit val4) map" where "simple_map_example = [IntV 1 \<mapsto> IntV 2]"
 
-abbreviation TV where "TV \<equiv> (TPrim TInt)"
+abbreviation MapTV where "MapTV \<equiv> MapV (TPrim TInt) (TPrim TInt)"  (* convenience for testing purposes *)
 
-abbreviation M1 where "M1 \<equiv> MapV TV TV [IntV 1 \<mapsto> IntV 2]"
-fun m1 where "m1 () = M1 (M1 undefined)"
+abbreviation m11 :: "unit val1" where "m11 \<equiv> MapTV [IntV 1 \<mapsto> IntV 2] None"
+abbreviation m12 :: "unit val2" where "m12 \<equiv> MapTV [IntV 1 \<mapsto> IntV 2] (Some m11)"
+abbreviation m13 :: "unit val3" where "m13 \<equiv> MapTV [IntV 1 \<mapsto> IntV 2] (Some m12)"
+abbreviation m14 :: "unit val4" where "m14 \<equiv> MapTV [IntV 1 \<mapsto> IntV 2] (Some m13)"
 
-abbreviation M2 where "M2 \<equiv> MapV TV TV [(M1 undefined) \<mapsto> IntV 4]"
-fun m2 :: "unit \<Rightarrow> unit val4" where "m2 () = M2 (M2 undefined)"
+abbreviation m22 :: "unit val2" where "m22 \<equiv> MapTV [m11 \<mapsto> IntV 4] None"
+abbreviation m23 :: "unit val3" where "m23 \<equiv> MapTV [m12 \<mapsto> IntV 4] (Some m22)"
+abbreviation m24 :: "unit val4" where "m24 \<equiv> MapTV [m13 \<mapsto> IntV 4] (Some m23)"
 
-abbreviation M3 where "M3 \<equiv> MapV TV TV [(M2 undefined) \<mapsto> IntV 6]"
-fun m3 :: "unit \<Rightarrow> unit val4" where "m3 () = M3 (M3 undefined)"
+abbreviation m33 :: "unit val3" where "m33 \<equiv> MapTV [m22 \<mapsto> IntV 6] None"
+abbreviation m34 :: "unit val4" where "m34 \<equiv> MapTV [m23 \<mapsto> IntV 6] (Some m33)"
 
-abbreviation MG where "MG \<equiv> MapV TV TV [(M2 undefined) \<mapsto> m1 ()]"
-fun mg :: "unit \<Rightarrow> unit val4" where "mg () = MG (MG undefined)"
+abbreviation mg3 :: "unit val3" where "mg3 \<equiv> MapTV [m22 \<mapsto> m13] None"
+abbreviation mg4 :: "unit val4" where "mg4 \<equiv> MapTV [m23 \<mapsto> m14] (Some mg3)"
 
-(* generic select function *)
-fun down :: "('a, _) val_aux \<Rightarrow> _" where
+(* generic MapV select function *)
+primrec down :: "('a, _) val_aux \<rightharpoonup> ('a, _) val_aux" where
     "down (MapV _ _ _ k) = k"
-  | "down (LitV v) = LitV v"
-  | "down (AbsV v) = AbsV v"
+  | "down (LitV v) = Some (LitV v)"
+  | "down (AbsV v) = Some (AbsV v)"
 
 fun select :: "('a, _) val_aux \<Rightarrow> ('a, _) val_aux \<rightharpoonup> ('a, _) val_aux" where
-    "select (MapV _ _ m _) k = m (down k)"
-  | "select _ _ = undefined"  
+    "select (MapV _ _ m _) k = Option.bind (down k) m"
+  | "select _ _ = None"
 
-lemma "select (mg ()) (m2 ()) = Some (m1 ())" by simp
-
-value [nbe] "[undefined \<mapsto> 1] undefined"
+lemma "select mg4 m24 = Some m14" by simp
 
 (* there needs to be as many additional store functions, as there are nesting levels *)
-fun store1 :: "('a, _) val_aux \<Rightarrow> ('a, _) val_aux \<Rightarrow> ('a, _) val_aux \<Rightarrow> ('a, _) val_aux" where
-    "store1 (MapV tk tv mm mk) k v = (MapV tk tv (mm(down k \<mapsto> v)) undefined)"
+(* user needs to generate these functions (is there a way to make this cleaner, macro?) *)
+fun store3 :: "('a, _) val_aux option \<Rightarrow> ('a, _) val_aux option \<Rightarrow> ('a, _) val_aux option \<rightharpoonup> ('a, _) val_aux" where
+    "store3 _ _ _ = None"
 
-fun store :: "('a, _) val_aux \<Rightarrow> ('a, _) val_aux \<Rightarrow> ('a, _) val_aux \<Rightarrow> ('a, _) val_aux" where
-    "store  (MapV tk tv mm mk) k v = (MapV tk tv (mm(down k \<mapsto> v)) (store1 mk (down k) (down v)))"
-  | "store _ _ _ = undefined"
+fun store2 :: "('a, _) val_aux option \<Rightarrow> ('a, _) val_aux option \<Rightarrow> ('a, _) val_aux option \<rightharpoonup> ('a, _) val_aux" where
+    "store2 (Some (MapV tk tv mm mk)) (Some k) (Some v) = Some (MapV tk tv (mm(k \<mapsto> v)) (store3 mk (down k) (down v)))"
+  | "store2 _ _ _ = None"
 
-lemma "select (store (mg ()) (m2 ()) (IntV 42)) (m2 ()) = Some (IntV 42)" by simp
+fun store1 :: "('a, _) val_aux option \<Rightarrow> ('a, _) val_aux option \<Rightarrow> ('a, _) val_aux option \<rightharpoonup> ('a, _) val_aux" where
+    "store1 (Some (MapV tk tv mm mk)) (Some k) (Some v) = Some (MapV tk tv (mm(k \<mapsto> v)) (store2 mk (down k) (down v)))"
+  | "store1 _ _ _ = None"
+
+fun store0 :: "('a, _) val_aux option \<Rightarrow> ('a, _) val_aux option \<Rightarrow> ('a, _) val_aux option \<rightharpoonup> ('a, _) val_aux" where
+    "store0 (Some (MapV tk tv mm mk)) (Some k) (Some v) = Some (MapV tk tv (mm(k \<mapsto> v)) (store1 mk (down k) (down v)))"
+  | "store0 _ _ _ = None"
+
+fun store :: "'a val4 \<Rightarrow> ('a, _) val_aux \<Rightarrow> ('a, _) val_aux \<rightharpoonup> ('a, _) val_aux" where
+    "store (MapV tk tv mm mk) k v = store0 (Some (MapV tk tv mm mk)) (down k) (Some v)"
+  | "store _ _ _ = None"
+
+
+primrec select_option where "select_option (Some v) k = select v k"
+lemma "select_option (store mg4 m24 (IntV 42)) m24 = Some (IntV 42)" by simp
 
 
 type_synonym 'a val = "'a val4"
